slight refactoring

Saturn/Solverstep.lean
@@ -158,4 +158,138 @@ def pullBackSolution{dom n: Nat}(branch: Bool)(focus : Nat)(focusLt : focus < n 
               ⟨skip focus i, skipPlusOne iw, lem6⟩
 
 
+def unitClause(n : Nat)(b : Bool)(k : Nat) (w : k < n + 1):   Clause (n + 1):=
+  insert (some b) n k w (contradiction n) 
+
+theorem unitDiag(n : Nat)(b : Bool)(k : Nat) (w : k < n + 1): 
+          unitClause n b k w k w = b :=
+          insertAtFocus (some b) n k w (contradiction n)
+
+theorem unitSkip(n : Nat)(b : Bool)(k : Nat) (w : k < n + 1): 
+          (i: Nat) → (iw : i < n) →  unitClause n b k w (skip k i) 
+                  (skipPlusOne iw) = none := fun i iw => 
+          insertAtImage (some b) n k w (contradiction n) i iw
+
+structure IsUnitClause{n: Nat}(clause: Clause (n +1)) where
+  index: Nat 
+  bound : index < n + 1
+  parity: Bool
+  equality : clause = unitClause n parity index bound
+
+def clauseUnit{n: Nat}(clause: Clause (n + 1)) : Option (IsUnitClause clause) :=
+  let f : Fin (n + 1) →   (Option (IsUnitClause clause)) := 
+    fun ⟨k, w⟩ =>
+      match deqSeq _ clause  (unitClause n true k w) with 
+      | isTrue pf => 
+        let cl : IsUnitClause clause := IsUnitClause.mk k w true pf 
+        some (cl)
+      | isFalse _ => 
+        match deqSeq _ clause  (unitClause n false k w) with 
+      | isTrue pf => 
+        let cl : IsUnitClause clause := IsUnitClause.mk k w false pf 
+        some (cl)
+      | isFalse _ => none  
+  let seq : FinSeq (n + 1) (Fin (n + 1)) := fun k w => ⟨k, w⟩
+  findSome? f seq
+
+structure SomeUnitClause{l n : Nat}(clauses : FinSeq l  (Clause (n + 1))) where
+  pos: Nat
+  posBound : pos < l
+  index: Nat 
+  bound : index < n + 1
+  parity: Bool
+  equality : clauses pos posBound = unitClause n parity index bound
+
+def someUnitClause {l : Nat} {n : Nat}: (clauses : FinSeq l  (Clause (n + 1))) →  
+  Option (SomeUnitClause clauses)  := 
+    match l with 
+    | 0 => fun  _ =>  none
+    | m + 1 => 
+      fun  cls =>
+        match clauseUnit (cls 0 (zeroLtSucc m)) with
+        | some u => some ⟨0, zeroLtSucc _, u.index, u.bound, u.parity, u.equality⟩ 
+        | none => 
+          let tcls := tail cls
+          let tail := someUnitClause  tcls
+          match tail with
+          | some ⟨i, w, index, bd, par, eql⟩ => 
+            some ⟨i + 1, leOfSuccLeSucc w, index, bd, par, eql⟩
+          | none => none
+
+structure HasPureVar{dom n : Nat}(clauses : FinSeq dom  (Clause n)) where
+  index : Nat
+  bound : index < n
+  parity : Bool
+  evidence : (k : Nat) → (lt : k < dom) → 
+          (clauses k lt index bound = none) ∨  (clauses k lt index bound = some parity)
+
+structure IsPureVar{dom n : Nat}(clauses : FinSeq dom  (Clause n))
+                      (index: Nat)(bound : index < n)(parity : Bool) where
+  evidence : (k : Nat) → (lt : k < dom) → (clauses k lt index bound = none) ∨ 
+                                (clauses k lt index bound = some parity)
+
+def varIsPure{n : Nat}(index: Nat)(bound : index < n)(parity : Bool) : 
+  (dom: Nat) →  (clauses : FinSeq dom  (Clause n)) → 
+    Option (IsPureVar clauses index bound parity) :=
+  fun dom =>
+  match dom with
+  | 0 => 
+    fun clauses =>
+      let evidence : (k : Nat) → (lt : k < 0) →  
+        (clauses k lt index bound = none) ∨ (clauses k lt index bound = some parity) := 
+          fun k lt => nomatch lt
+      some ⟨evidence⟩
+  | m + 1 => 
+      fun clauses =>
+        let head := clauses 0 (zeroLtSucc _) index bound
+        if c : (head = none) ∨  (head = some parity) then
+          let tailSeq  := tail clauses
+          (varIsPure index bound parity _ tailSeq).map (
+            fun ⟨ tpf ⟩ =>
+              let pf : (j : Nat) → (w : j < (m +1)) → 
+                (clauses j w index bound = none) ∨ (clauses j w index bound = some parity) := 
+                fun j =>
+                  match j with 
+                  | 0 => fun w => c
+                  | i + 1 => fun w =>
+                    let tailWit : i < m := leOfSuccLeSucc w 
+                    tpf i tailWit
+              ⟨ pf ⟩
+          )
+        else none
+
+def findPureAux{n : Nat} : (dom: Nat) →  (clauses : FinSeq dom (Clause (n +1))) → 
+  (ub: Nat) → (lt : ub < n + 1) → 
+      Option (HasPureVar clauses) :=
+      fun dom clauses ub => 
+        match ub with
+        | 0 =>
+          fun lt =>
+           ((varIsPure 0 lt true dom clauses).map (
+            fun ⟨evidence⟩ =>
+              HasPureVar.mk 0 lt true evidence
+              )).orElse (
+                (varIsPure 0 lt false dom clauses).map (
+            fun ⟨evidence⟩ =>
+              HasPureVar.mk 0 lt false evidence
+              )
+              )
+        | l + 1 =>
+          fun lt =>
+            ((findPureAux dom clauses l (leStep lt)).orElse (              
+              (varIsPure l (leStep lt) true dom clauses).map (
+            fun ⟨evidence⟩ =>
+              HasPureVar.mk l (leStep lt) true evidence
+              )
+              )).orElse (              
+              (varIsPure l (leStep lt) false dom clauses).map (
+            fun ⟨evidence⟩ =>
+              HasPureVar.mk l (leStep lt) false evidence
+              )
+              )
+            
+def hasPure{n : Nat}{dom: Nat}(clauses : FinSeq dom  (Clause (n +1))) 
+             : Option (HasPureVar clauses) :=
+          findPureAux dom clauses n (Nat.leRefl _)
+
 
